\documentclass[11pt]{article}
\usepackage{geometry}
 \geometry{
 letterpaper,
 left=1in,
 right=1in,
 top=1in,
 bottom=1in
 }
\usepackage[utf8]{inputenc}

\usepackage[super,sort&compress,numbers]{natbib}
\bibliographystyle{naturemag}
%\bibliographystyle{plainnat} %abbrv, acm, alpha, apalike, ieeetr, plain, siam, unsrt
\usepackage{url}
\urlstyle{same}
\usepackage{color}
\usepackage{graphicx}
\usepackage{longtable}
\usepackage{setspace}
\usepackage[skip=10pt, indent=20pt]{parskip}
\usepackage{changepage}
\usepackage[normalem]{ulem}
\usepackage{arydshln}
\usepackage[font=small] {caption}
\usepackage{subcaption}
\usepackage{chngcntr}
\usepackage{wrapfig}
\usepackage{sidecap}
\sidecaptionvpos{figure}{c} 
\usepackage{amsmath,amssymb,amsthm} % AMS styles for extra equation formatting
\usepackage{cleveref}
\renewcommand\thesection{\Roman{section}}
\renewcommand\thesubsection{\thesection.\arabic{subsection}}
\begin{document}

\section{An attempt at a slightly different derivation for our probability problem}

\section{Probability Problem Statement}

Consider the following setup:
\begin{itemize}
    \item There are two sets of objects: $ S $ with size $ n_S $ and $ I $ with size $ n_I $, where $ n_S, n_I > 0 $.
    \item There is a set $ G $ of locations, with size $ n_G $.
    \item Each object from both $ S $ and $ I $ is independently placed at location $ G_i $ with probability $ w_i $.
    \item If at least one object from $ S $ and at least one object from $ I $ are placed at the same location $ G_i $, an event $ E $ occurs at $ G_i $ with probability $ \epsilon_i $.
\end{itemize}

We derive:
\begin{enumerate}
    \item The probability that $ E $ occurs at a specific location $ i $.
    \item The probability that $ E $ occurs at least once at any location in $ G $.
\end{enumerate}

We consider three cases:
\begin{enumerate}
    \item General case: Any $ n_I $ and any $ n_S $.
    \item Special case: $ n_I = 1 $, any $ n_S $.
    \item Special case: $ n_I = 1 $, $ n_S = 1 $.
\end{enumerate}

\section{General Case: Any $ n_I $ and $ n_S $}

\subsection{Probability of $ E $ at Location $ i $}

Define $ S_i $ and $ I_i $ as the number of objects from $ S $ and $ I $ that land at location $ G_i $. Since each object chooses $ G_i $ with probability $ w_i $, we have:

\begin{equation}
S_i \sim \text{Binomial}(n_S, w_i), \quad I_i \sim \text{Binomial}(n_I, w_i).
\end{equation}

The probability that at least one object from $ S $ and at least one object from $ I $ land at $ G_i $ is:

\begin{equation}
P(S_i \geq 1, I_i \geq 1) = 1 - P(S_i = 0) - P(I_i = 0) + P(S_i = 0, I_i = 0).
\end{equation}

Since the binomial probability mass function gives:

\begin{equation}
P(S_i = 0) = (1 - w_i)^{n_S}, \quad P(I_i = 0) = (1 - w_i)^{n_I},
\end{equation}

and since placements are independent,

\begin{equation}
P(S_i = 0, I_i = 0) = P(S_i = 0) P(I_i = 0) = (1 - w_i)^{n_S + n_I}.
\end{equation}

Thus,

\begin{equation}
P(S_i \geq 1, I_i \geq 1) = 1 - (1 - w_i)^{n_S} - (1 - w_i)^{n_I} + (1 - w_i)^{n_S + n_I}.
\end{equation}

Given this overlap, $ E $ occurs with probability $ \epsilon_i $, so:

\begin{equation}
P(E_i) = \epsilon_i \left[ 1 - (1 - w_i)^{n_S} - (1 - w_i)^{n_I} + (1 - w_i)^{n_S + n_I} \right].
\end{equation}

\subsection{Probability of $ E $ at Any Location}

Since locations are independent, the probability that $ E $ does not occur at any location is:

\begin{equation}
\prod_{i=1}^{n_G} \left( 1 - P(E_i) \right).
\end{equation}

Thus, the probability that $ E $ occurs at least once is:

\begin{equation}
P(E_{\text{any}}) = 1 - \prod_{i=1}^{n_G} \left( 1 - P(E_i) \right).
\end{equation}

\section{Special Case: $ n_I = 1 $, Any $ n_S $}

\subsection{Probability of $ E $ at Location $ i $}

Setting $ n_I = 1 $ in the general formula:

\begin{equation}
P(E_i) = \epsilon_i \left[ 1 - (1 - w_i)^{n_S} - (1 - w_i) + (1 - w_i)^{n_S + 1} \right].
\end{equation}

Rearranging terms:

\begin{equation}
P(E_i) = \epsilon_i \left[ w_i - (1 - w_i)^{n_S} + (1 - w_i)^{n_S + 1} \right].
\end{equation}

Factoring:

\begin{equation}
P(E_i) = \epsilon_i w_i \left[ 1 - (1 - w_i)^{n_S} \right].
\end{equation}

\subsection{Probability of $ E $ at Any Location}

\begin{equation}
P(E_{\text{any}}) = 1 - \prod_{i=1}^{n_G} \left( 1 - \epsilon_i w_i \left( 1 - (1 - w_i)^{n_S} \right) \right).
\end{equation}

\section{Special Case: $ n_I = 1 $, $ n_S = 1 $}

\subsection{Probability of $ E $ at Location $ i $}

If $ n_I = 1 $ and $ n_S = 1 $, we substitute into the previous formula:

\begin{equation}
P(E_i) = \epsilon_i w_i \left[ 1 - (1 - w_i) \right].
\end{equation}

Since $ 1 - (1 - w_i) = w_i $, we get:

\begin{equation}
P(E_i) = \epsilon_i w_i^2.
\end{equation}

\subsection{Probability of $ E $ at Any Location}

\begin{equation}
P(E_{\text{any}}) = 1 - \prod_{i=1}^{n_G} \left( 1 - \epsilon_i w_i^2 \right).
\end{equation}


\end{document}